proof_of_soundness/ConfigVars.v
@@ -4,9 +4,11 @@ Require Import Coq.Lists.List.
 
 From Cpp2C Require Import Syntax.
 
+
 (* Environment and store/state are implemented as associative arrays. *)
 Definition environment : Set := @list (string * nat).
 Definition state : Set := @list (nat * Z).
+
 
 (* Looks up a variable name in the environment and returns
    the corresponding L-value wrapped in an option type if found;
@@ -14,34 +16,28 @@ Definition state : Set := @list (nat * Z).
 Definition lookupE (x:string) (E:environment) : option nat :=
   option_map snd (find (fun pair => String.eqb (fst pair) x) E).
 
+
 (* Looks up an L-value in the store and returns
    the corresponding R-value wrapped in an option type if found;
-   otherwise returns None *)
+   otherwise returns None                              *)
 Definition lookupS (l:nat) (S:state) : option Z :=
   option_map snd (find (fun pair => Nat.eqb (fst pair) l) S).
 
 
 (* Mappings from function and macro names to their definitions *)
 (* Functions are defined as a 3-tuple:
-   0: Environment which contains processed local declarations and
-      parameters
+   0: Parameter names
    1: Body that is a statement (could be a compound statement)
    2: Return expression *)
-(* TODO: Eventually we may want to swap the environment out for a
-         parameter list and operate on that instead *)
-Definition func_definition : Set := ((stmt) * expr).
+Definition func_definition : Set := ((list string) * stmt * expr).
 Definition func_definitions : Set := @list (string * func_definition).
 
+
 (* Macro definitions are serialized as a two-tuple containing
-   the macros parameters mapped to their arguments (the environment)
-   and the macro body (a single expression).
-   TODO: This does not exactly model how macros work. To fix this,
-         we will need to swap out the environment for a list of
-         parameters and the body for something more akin to what we
-         have for functions.
-   *)
-Definition macro_definition : Set := (expr).
+   the macros parameters and the macro body (a single expression) *)
+Definition macro_definition : Set := (list (string) * expr).
 Definition macro_definitions : Set := @list (string * macro_definition).
+
 
 (* Looks up a function name in the function defintion list and returns
    the corresponding definition wrapped in an option type if found;
@@ -49,6 +45,7 @@ Definition macro_definitions : Set := @list (string * macro_definition).
 Definition definition
   (defs:func_definitions) (x:string) : option func_definition :=
   option_map snd (find (fun pair => String.eqb (fst pair) x) defs).
+
 
 (* Looks up a macro name in the function defintion list and returns
    the corresponding definition wrapped in an option type if found;
